vType: swap {restr}Frame{,2}; coercePaintingType reqd
Converting everything to the first definition lets us make progress
throughout, but Painting fundamentally does not compute on the first
definition, making it impossible to define RestrPainting. We need to
phrase RestrPainting in terms of the first definition, but convert to
the CohFrameTypesAndRestrFrames definition when doing the proof. The
first step is to define coercePaintingType, for which we start to make
progress.

theories/νType/νType.v
@@ -308,36 +308,37 @@ Definition mkCohFramesFromFull: forall p {Hp: p.+1 <~ n.+2},
     with 0 => fun _ => I | p.+1 => fun Hp => (aux p.+1 Hp).1 end Hp
   end.
 
-(** RestrFrames(n+2,p) from full CohFrames, going down via CohFrames *)
-Definition RestrFrames p {Hp: p.+1 <~ n.+2} :=
-  ((mkCohFrameTypesAndRestrFrames p (Hp := Hp)).(RestrFramesDef)
-    (mkCohFramesFromFull p (Hp := Hp))).
 
 (** RestrFrames(n+2,p) from full CohFrames, going down via RestrFrames *)
-Definition RestrFrames2 p {Hp: p.+1 <~ n.+2} :=
+Definition RestrFrames p {Hp: p.+1 <~ n.+2} :=
   mkRestrFramesFromFull n.+1 Frame' Painting' mkFullRestrFrames p.+1
     (Hp := Hp).
+
+(** RestrFrames(n+2,p) from full CohFrames, going down via CohFrames *)
+Definition RestrFrames2 p {Hp: p.+1 <~ n.+2} :=
+  ((mkCohFrameTypesAndRestrFrames p (Hp := Hp)).(RestrFramesDef)
+    (mkCohFramesFromFull p (Hp := Hp))).
 
 Lemma eqRestrFramesDef {p} {Hp: p.+1 <~ n.+2}:
   RestrFrames p (Hp := Hp) = RestrFrames2 p.
 Proof.
   induction Hp using leI_rectD. now easy. simpl in IHHp.
   clear p; rename p0 into p. unfold RestrFrames, RestrFrames2 in *.
-  simpl. now rewrite <- IHHp.
+  simpl. now rewrite IHHp.
 Defined.
 
-(** Frame(n+2,p) from full CohFrames, going down via CohFrames *)
+(** Frame(n+2,p) from full CohFrames, going down via RestrFrames *)
 Definition Frame p {Hp: p <~ n.+2} :=
+  mkFrame n.+1 Frame' Painting' mkFullRestrFrames p (Hp := Hp).
+
+(** Frame(n+2,p) from full CohFrames, going down via CohFrames *)
+Definition Frame2 p {Hp: p <~ n.+2} :=
   FrameOfRestrFrames p
     (match Hp in p <~ _ return (mkRestrFrameTypesAndFrames n.+1 Frame' Painting'
       p).(RestrFrameTypesDef) with
-    | leI_refl _ => RestrFrames n.+1 (Hp := leI_refl _)
-    | @leI_down _ p Hp => (RestrFrames p (Hp := Hp)).1
+    | leI_refl _ => RestrFrames2 n.+1 (Hp := leI_refl _)
+    | @leI_down _ p Hp => (RestrFrames2 p (Hp := Hp)).1
     end).
-
-(** Frame(n+2,p) from full CohFrames, going down via RestrFrames *)
-Definition Frame2 p {Hp: p <~ n.+2} :=
-  mkFrame n.+1 Frame' Painting' mkFullRestrFrames p (Hp := Hp).
 
 Lemma eqFrameDef {p} {Hp: p <~ n.+2}:
   Frame p (Hp := Hp) = Frame2 p (Hp := Hp).
@@ -348,20 +349,20 @@ Proof.
     (Hp := leI_down Hp)).(FrameDef)) x.1) (eqRestrFramesDef (Hp := Hp))).
 Defined.
 
-(** RestrFrame(n+2,p) from full CohFrames,  going down via CohFrames *)
+(** RestrFrame(n+2,p) from full CohFrames, going down via RestrFrames *)
 Definition RestrFrame p {Hp: p.+1 <~ n.+2} q {Hpq: p <~ q} {Hq: q <~ n.+1}
   ε (d: Frame p): Frame' p (Hp := leI_lower_both Hp) :=
   (RestrFrames p (Hp := Hp)).2 q Hpq Hq ε d.
 
-(** RestrFrame(n+2,p) from full CohFrames, going down via RestrFrames *)
+(** RestrFrame(n+2,p) from full CohFrames, going down via CohFrames *)
 Definition RestrFrame2 p {Hp: p.+1 <~ n.+2} q {Hpq: p <~ q} {Hq: q <~ n.+1}
-  ε (d: Frame p): Frame' p (Hp := leI_lower_both Hp) :=
-  (RestrFrames2 p (Hp := Hp)).2 q Hpq Hq ε (rew eqFrameDef in d).
+  ε (d: Frame2 p): Frame' p (Hp := leI_lower_both Hp) :=
+  (RestrFrames2 p (Hp := Hp)).2 q Hpq Hq ε d.
 
 Lemma eqRestrFrameDef {p} {Hp: p.+1 <~ n.+2} {q} {Hpq: p <~ q}
   {Hq: q <~ n.+1} {ε} {d: Frame p}:
   RestrFrame p q (Hpq := Hpq) (Hq := Hq) ε d =
-  RestrFrame2 p q (Hp := Hp) (Hpq := Hpq) (Hq := Hq) ε d.
+  RestrFrame2 p q (Hp := Hp) (Hpq := Hpq) (Hq := Hq) ε (rew eqFrameDef in d).
 Proof.
   unfold RestrFrame, RestrFrame2, eqFrameDef.
   rewrite <- rew_map with (f := fun x => (mkRestrFrameTypesAndFrames n.+1 Frame'
@@ -378,17 +379,22 @@ Definition mkCohFrameFromFull p {Hp: p.+2 <~ n.+2} r q {Hpr: p.+1 <~ r.+1}
   RestrFrame' p r (Hpq := leI_lower_both Hpr) (Hq := leI_lower_both Hr) ω
     (RestrFrame p q.+1 (Hpq := leI_down (leI_trans Hpr Hrq)) (Hq := Hq) ε d).
 Proof.
-  now exact ((mkCohFramesFromFull p.+1).2 r q Hpr Hrq Hr Hq ε ω d).
+  repeat rewrite eqRestrFrameDef.
+  now exact ((mkCohFramesFromFull p.+1).2 r q Hpr Hrq Hr Hq ε ω
+    (rew eqFrameDef in d)).
 Defined.
 
 Definition CohFrame {p} {Hp: p.+2 <~ n.+2} r q {Hpr Hrq Hr Hq} :=
   mkCohFrameFromFull p (Hp := Hp) r q (Hpr := Hpr) (Hrq := Hrq) (Hr := Hr)
     (Hq := Hq).
 
-Let coerceFrameSpType {p} {Hp: p.+1 <~ n.+2} := {d: Frame p &T
-  forall ε, Painting' p (RestrFrame p p (Hp := Hp)
+Definition Painting p {Hp: p <~ n.+2} {E: Frame n.+2 -> HSet} :=
+  mkPainting n.+1 Frame' Painting' mkFullRestrFrames p (Hp := Hp) (E := E).
+
+Let coerceFrameSpType {p} {Hp: p.+1 <~ n.+2} := {d: Frame2 p &T
+  forall ε, Painting' p (RestrFrame2 p p (Hp := Hp)
   (Hpq := leI_lower_both (leI_refl _)) (Hq := leI_lower_both Hp) ε d)} ->
-  Frame p.+1 (Hp := Hp).
+  Frame2 p.+1 (Hp := Hp).
 
 Definition coerceFrameSp {p} {Hp: p.+1 <~ n.+2}: coerceFrameSpType :=
   match Hp in S_p <~ _ return
@@ -404,17 +410,33 @@ Definition coerceFrameSp {p} {Hp: p.+1 <~ n.+2}: coerceFrameSpType :=
     with 0 => fun _ => I | p.+1 => fun Hp => id end Hp
   end.
 
-Definition Painting p {Hp: p <~ n.+2} {E: Frame n.+2 -> HSet} :=
+Definition Painting2 p {Hp: p <~ n.+2} {E: Frame2 n.+2 -> HSet} :=
   (fix aux p Hp :=
-  match Hp in p <~ _ return Frame (Hp := Hp) p -> HSet with
+  match Hp in p <~ _ return Frame2 (Hp := Hp) p -> HSet with
  | leI_refl _ => E
  | @leI_down _ p Hp => fun d =>
-    {l: hforall ε, Painting' p (RestrFrame p p ε d) &
+    {l: hforall ε, Painting' p (RestrFrame2 p p ε d) &
       (aux p.+1 Hp) (coerceFrameSp (d; l))}
 end) p Hp.
 
-Lemma RestrPainting p {Hp: p.+1 <~ n.+2}
-  {E: Frame n.+2 (Hp := leI_refl _) -> HSet}:
+Lemma pi1_eq {A A': HSet} (p: A = A') (u: A -> HSet): A' -> HSet.
+Proof.
+  now easy.
+Qed.
+
+Definition coercePaintingType {p} {Hp: p.+1 <~ n.+2}
+  {E: Frame n.+2 -> HSet} {d: Frame p}:
+  Painting p (Hp := leI_down Hp) (E := E) d ->
+  Painting2 p (Hp := leI_down Hp) (E := pi1_eq eqFrameDef E)
+    (rew eqFrameDef in d).
+Proof.
+  unfold Painting, Painting2. induction Hp using leI_rectD.
+  - intros H; simpl in H; unshelve eapply existT. intros ε.
+    rewrite <- eqRestrFrameDef. admit. admit.
+  - intros H. admit.
+Admitted.
+
+Lemma RestrPainting p {Hp: p.+1 <~ n.+2} {E: Frame n.+2 -> HSet}:
     forall q (Hpq: p <~ q) (Hq: q <~ n.+1) ε (d: Frame p),
   Painting p (Hp := leI_down Hp) (E := E) d ->
   Painting' p (RestrFrame p q (Hpq := Hpq) (Hq := Hq) ε d).
@@ -433,8 +455,8 @@ Proof.
     now exact (rew [Painting'' p] CohFrame p q (Hpr := leI_refl _) ε ω d in
       RestrPainting' p q ε (RestrFrame p p ω d) (c.1 ω)).
     set (l := c.2).
-    now apply (IHHpq (leI_raise_both (leI_trans Hpq Hq)) Hq _) in l.
-Defined.
+    apply (IHHpq (leI_raise_both (leI_trans Hpq Hq)) Hq _) in l.
+Admitted.
 
 End CohFramesDef.
 
@@ -463,7 +485,6 @@ End CohFramesDef.
     depends on paintings at level n-1 and n-2; just as we have frame' and
      frame'', we have painting' and painting''. *)
 
-Set Printing Implicit.
 Class νTypeAux n := {
   frame'' p {Hp: p <~ n}: HSet;
   painting'' p {Hp: p <~ n}: frame'' p -> HSet;
@@ -603,18 +624,13 @@ Instance mkνType {n} {C: νType n}: νType n.+1.
 Proof.
   unshelve esplit.
   now apply mkPrefix'.
-  intro D.
   unshelve esplit.
   now eapply mkFrame''.
   now eapply mkPainting''.
   now eapply mkRestrFrames'.
-  intros E' p q Hp Hpq Hq.
-  replace Hp with (leI_trans (leI_raise_both Hpq) (leI_raise_both Hq))
-    by apply leI_irrelevance.
-  intros ε d X.
-  apply (mkRestrPainting' n C D p q ε).
-  Show.
-Admitted.
+  now eapply mkRestrPainting'.
+  now eapply mkCohFrames.
+Qed.
 
 Definition mkCohLayer {n} {C: νType n} {p r q} {Hpr: p.+3 <= r.+3}
   {Hrq: r.+3 <= q.+3} {Hq: q.+3 <= n.+1} {ε ω}
